[WIP] Ranged integer experiments

src/ir/ast.rs
@@ -5,8 +5,8 @@ use std::rc::Rc;
 
 use name::Named;
 pub use syntax::ast::Field;
-pub use syntax::ast::host::{Binop, Const, IntSuffix, TypeConst, Unop};
-pub use syntax::ast::host::{FloatType, SignedType, UnsignedType};
+pub use syntax::ast::host::{Binop, Const, TypeConst, Unop};
+pub use syntax::ast::host::{FloatType, IntType};
 pub use syntax::ast::binary::{Endianness, TypeConst as BinaryTypeConst};
 use var::{ScopeIndex, Var};
 
