experiments/lean/src/ddl/host/arith.lean
@@ -1,0 +1,175 @@
+/- A sublanguage of bounded integer arithmetic expressions -/
+namespace ddl.host.arith
+
+  /- Unary operators -/
+  inductive unop : Type
+    | neg : unop
+
+  /- Binary operators -/
+  inductive binop : Type
+    | add : binop
+    | sub : binop
+    | mul : binop
+
+  /- Integer arithmetic expressions -/
+  inductive expr : Type
+    | const : ℤ → expr
+    | unop : unop → expr → expr
+    | binop : binop → expr → expr → expr
+
+  namespace expr
+
+    instance : has_coe ℤ expr := ⟨const⟩
+    instance : has_neg expr := ⟨unop unop.neg⟩
+    instance : has_add expr := ⟨binop binop.add⟩
+    instance : has_sub expr := ⟨binop binop.sub⟩
+    instance : has_mul expr := ⟨binop binop.mul⟩
+
+  end expr
+
+
+  /- Bounded integer arithemetic types -/
+  structure type : Type :=
+    (min : ℤ)
+    (max : ℤ)
+    (min_le_max : min ≤ max)
+
+  namespace type
+
+    def const (n : ℤ) : type :=
+      { min := n
+      , max := n
+      , min_le_max := by refl
+      }
+
+    private lemma neg_le_int {a b : ℤ} (h : b ≤ a) : -a ≤ -b :=
+      by admit
+
+    def neg (t₁ : type) : type :=
+      { min := -t₁.max
+      , max := -t₁.min
+      , min_le_max := neg_le_int t₁.min_le_max
+      }
+
+    private lemma add_le_int {a₁ a₂ b₁ b₂ : ℤ} (h₁ : a₁ ≤ b₁) (h₂ : a₂ ≤ b₂) : a₁ + a₂ ≤ b₁ + b₂ :=
+      by admit
+
+    def add (t₁ t₂ : type) : type :=
+      { min := t₁.min + t₂.min
+      , max := t₁.max + t₂.max
+      , min_le_max := add_le_int t₁.min_le_max t₂.min_le_max
+      }
+
+    private lemma sub_le_int {a₁ a₂ b₁ b₂ : ℤ} (h₁ : a₁ ≤ b₁) (h₂ : a₂ ≤ b₂) : a₁ - a₂ ≤ b₁ - b₂ :=
+      by admit
+
+    def sub (t₁ t₂ : type) : type :=
+      { min := t₁.min - t₂.min
+      , max := t₁.max - t₂.max
+      , min_le_max := sub_le_int t₁.min_le_max t₂.min_le_max
+      }
+
+    def mul (t₁ t₂ : type) : type :=
+      sorry
+
+    instance : has_neg type := ⟨neg⟩
+    instance : has_add type := ⟨add⟩
+    instance : has_sub type := ⟨sub⟩
+    instance : has_mul type := ⟨mul⟩
+
+  end type
+
+
+  /- Typing relation for integer arithmetic -/
+  inductive has_type : expr → type → Type
+    | const {n : ℤ} :
+        has_type n (type.const n)
+    | unop_neg {e₁ t₁} :
+        has_type e₁ t₁ →
+        has_type (-e₁) (-t₁)
+    | binop_add {e₁ e₂ t₁ t₂} :
+        has_type e₁ t₁ →
+        has_type e₂ t₂ →
+        has_type (e₁ + e₂) (t₁ + t₂)
+    | binop_sub {e₁ e₂ t₁ t₂} :
+        has_type e₁ t₁ →
+        has_type e₂ t₂ →
+        has_type (e₁ - e₂) (t₁ - t₂)
+    | binop_mul {e₁ e₂ t₁ t₂} :
+        has_type e₁ t₁ →
+        has_type e₂ t₂ →
+        has_type (e₁ * e₂) (t₁ * t₂)
+    | subsume {e₁} {t₁ t₁' : type} :
+        has_type e₁ t₁ →
+        t₁'.min ≤ t₁.min →
+        t₁.max ≤ t₁'.max →
+        has_type e₁ t₁'
+    | coerce {e₁} {t₁ t₁' : type} :
+        has_type e₁ t₁ →
+        t₁.min ≤ t₁'.min →
+        t₁'.max ≤ t₁.max →
+        has_type e₁ t₁'
+
+  /- Small step evaluation -/
+
+  inductive value : expr → Prop
+    | const (n : ℤ) : value (expr.const n)
+
+  reserve infixl ` ⟹ `:50
+
+  inductive step : expr → expr → Prop
+    infixl ` ⟹ ` := step
+
+    | value {e} :
+        value e →
+        e ⟹ e
+    | unnop_neg {n₁} :
+        -(expr.const n₁) ⟹ expr.const (-n₁)
+    | unop_rec {op e₁ e₁'} :
+        e₁ ⟹ e₁' →
+        expr.unop op e₁ ⟹ expr.unop op e₁'
+    | binop_rec_l {op e₁ e₁' e₂} :
+        e₁ ⟹ e₁' →
+        expr.binop op e₁ e₂ ⟹ expr.binop op e₁' e₂
+    | binop_rec_r {op e₁ e₂ e₂'} :
+        value e₁ →
+        e₂ ⟹ e₂' →
+        expr.binop op e₁ e₂ ⟹ expr.binop op e₁ e₂'
+    | binop_add {n₁ n₂} :
+        expr.const n₁ + expr.const n₂ ⟹ expr.const (n₁ + n₂)
+    | binop_sub {n₁ n₂} :
+        expr.const n₁ - expr.const n₂ ⟹ expr.const (n₁ - n₂)
+    | binop_mul {n₁ n₂} :
+        expr.const n₁ * expr.const n₂ ⟹ expr.const (n₁ * n₂)
+
+  infixl ` ⟹ ` := step
+
+  -- PROGRESS
+  -- https://softwarefoundations.cis.upenn.edu/plf-current/StlcProp.html#lab220
+
+  theorem progress :
+      Π (e : expr) (t : type),
+      has_type e t →
+      value e ∨ ∃ e', e ⟹ e' :=
+    begin
+      intros e t ht,
+      -- TODO
+      admit
+    end
+
+
+  -- PRESERVATION
+  -- https://softwarefoundations.cis.upenn.edu/plf-current/StlcProp.html#lab222
+
+  theorem preservation :
+      Π (e e' : expr) (t : type),
+      has_type e t →
+      e ⟹ e' →
+      has_type e' t :=
+    begin
+      intros e e' t ht hs,
+      -- TODO
+      admit
+    end
+
+end ddl.host.arith
