experiments/lean/src/ddl/host/default.lean
@@ -1,3 +1,4 @@
+import ddl.host.arith
 import ddl.host.basic
 import ddl.host.evaluation
 import ddl.host.typing
